theories/Core/KTreeBasicFacts.v
@@ -1,3 +1,7 @@
+(** * Facts about the cocartesian category of KTrees *)
+
+(** Proofs about [loop] are separate, in [ITree.Core.KTreeFacts]. *)
+
 (* begin hide *)
 From Coq Require Import
      Morphisms.
@@ -6,7 +10,9 @@ From Paco Require Import paco.
 
 From ITree Require Import
      Basics.Basics
-     Basics.CategoryOps
+     Basics.Category
+     Basics.Function
+     Basics.FunctionFacts
      Core.ITreeDefinition
      Core.KTree
      Eq.UpToTausEquivalence.
@@ -15,41 +21,281 @@ Import ITreeNotations.
 Import CatNotations.
 Local Open Scope itree_scope.
 Local Open Scope cat_scope.
-Local Opaque paco2.
+
+Local Opaque ITree.bind' eutt eq_itree.
 (* end hide *)
 
 Global Instance Equivalence_eq_ktree {E A B} : @Equivalence (ktree E A B) eq2.
 Proof.
-  split.
-  - intros ab a; reflexivity.
-  - intros ab ab' eqAB a; symmetry; auto.
-  - intros ab ab' ab'' eqAB eqAB' a; etransitivity; eauto.
+  split; repeat intro.
+  - reflexivity.
+  - symmetry; auto.
+  - etransitivity; eauto.
 Qed.
 
-(* Facts about [loop] *)
+Section UnfoldLemmas.
 
-Notation loop_once_ f loop_ :=
-  (loop_once f (fun cb => Tau (loop_ f%function cb))).
-
-Lemma unfold_loop'' {E A B C} (f : C + A -> itree E (C + B)) (x : C + A) :
-    observe (loop_ f x)
-  = observe (loop_once f (fun cb => Tau (loop_ f cb)) x).
-Proof. reflexivity. Qed.
-
-Lemma unfold_loop' {E A B C} (f : C + A -> itree E (C + B)) (x : C + A) :
-    loop_ f x
-  ≅ loop_once f (fun cb => Tau (loop_ f cb)) x.
+Lemma assoc_l_itree {E A B C} (x : A + (B + C)) :
+  assoc_l_ A B C x ≅ @lift_ktree E (A + (B + C)) _ assoc_l x.
 Proof.
-  rewrite itree_eta, (itree_eta (loop_once _ _ _)).
+  cbv; destruct x as [ | [] ]; try rewrite bind_ret; reflexivity.
+Qed.
+
+Lemma assoc_r_itree {E A B C} (x : (A + B) + C) :
+  assoc_r_ A B C x ≅ @lift_ktree E ((A + B) + C) _ assoc_r x.
+Proof.
+  cbv; destruct x as [ [] | ]; try rewrite bind_ret; reflexivity.
+Qed.
+
+Lemma assoc_l_ktree {E A B C} :
+  assoc_l ⩯ @lift_ktree E (A + (B + C)) _ assoc_l.
+Proof.
+  cbv; intros [ | [] ]; try rewrite bind_ret; reflexivity.
+Qed.
+
+Lemma assoc_r_ktree {E A B C} :
+  assoc_r ⩯ @lift_ktree E ((A + B) + C) _ assoc_r.
+Proof.
+  intros ?; rewrite <- assoc_r_itree; reflexivity.
+Qed.
+
+End UnfoldLemmas.
+
+(** ** Equations *)
+
+Section CategoryLaws.
+
+Context {E : Type -> Type}.
+
+(** *** [compose_ktree] respect eq_ktree *)
+Global Instance eq_ktree_compose {A B C} :
+  @Proper (ktree E A B -> ktree E B C -> _) (eq2 ==> eq2 ==> eq2) cat.
+Proof.
+  intros ab ab' eqAB bc bc' eqBC.
+  intro a.
+  unfold cat, Cat_ktree, ITree.cat.
+  rewrite (eqAB a).
+  apply eutt_bind; try reflexivity.
+  intro b; rewrite (eqBC b); reflexivity.
+Qed.
+
+(** *** [compose_ktree] is associative *)
+Global Instance CatAssoc_ktree : CatAssoc (ktree E).
+Proof.
+  intros A B C D f g h a.
+  unfold cat, Cat_ktree, ITree.cat.
+  rewrite bind_bind.
   reflexivity.
 Qed.
 
-Lemma unfold_loop {E A B C} (f : C + A -> itree E (C + B)) (x : C + A) :
-    loop_ f x
-  ≈ loop_once f (loop_ f) x.
+(** *** [id_ktree] respect identity laws *)
+Global Instance CatIdL_ktree : CatIdL (ktree E).
 Proof.
-  rewrite unfold_loop'.
-  apply eutt_bind; try reflexivity.
-  intros []; try reflexivity.
-  rewrite tau_eutt; reflexivity.
+  intros A B f a; unfold cat, Cat_ktree, ITree.cat, id_, Id_ktree.
+  rewrite bind_ret. reflexivity.
 Qed.
+
+Global Instance CatIdR_ktree : CatIdR (ktree E).
+Proof.
+  intros A B f a; unfold cat, Cat_ktree, ITree.cat, id_, Id_ktree.
+  rewrite <- (bind_ret2 (f a)) at 2.
+  reflexivity.
+Qed.
+
+Global Instance Category_ktree : Category (ktree E).
+Proof.
+  constructor; typeclasses eauto.
+Qed.
+
+Global Instance InitialObject_ktree : InitialObject (ktree E) void.
+Proof. intros A f []. Qed.
+
+End CategoryLaws.
+
+(** *** [lift] properties *)
+
+Section LiftLaws.
+
+Context {E : Type -> Type}.
+
+Local Open Scope cat.
+
+(** *** [lift_ktree] is well-behaved *)
+
+Global Instance eq_lift_ktree {A B} :
+  Proper (eq2 ==> eq2) (@lift_ktree E A B).
+Proof.
+  repeat intro.
+  unfold lift_ktree.
+  erewrite (H a); reflexivity.
+Qed.
+
+Lemma lift_ktree_id {A: Type}: (id_ A ⩯ @lift_ktree E A A (id_ A))%cat.
+Proof.
+  reflexivity.
+Qed.
+
+Fact compose_lift_ktree {A B C} (ab : A -> B) (bc : B -> C) :
+  (@lift_ktree E _ _ ab >>> lift_ktree bc ⩯ lift_ktree (ab >>> bc))%cat.
+Proof.
+  intros a.
+  unfold lift_ktree, cat, Cat_ktree, ITree.cat.
+  rewrite bind_ret_.
+  reflexivity.
+Qed.
+
+Fact compose_lift_ktree_l {A B C D} (f: A -> B) (g: B -> C) (k: ktree E C D) :
+  (lift_ktree f >>> (lift_ktree g >>> k) ⩯ lift_ktree (g ∘ f) >>> k)%cat.
+Proof.
+  rewrite <- cat_assoc.
+  rewrite compose_lift_ktree.
+  reflexivity.
+  typeclasses eauto.
+Qed.
+
+Fact compose_lift_ktree_r {A B C D} (f: B -> C) (g: C -> D) (k: ktree E A B) :
+  ((k >>> lift_ktree f) >>> lift_ktree g ⩯ k >>> lift_ktree (g ∘ f))%cat.
+Proof.
+  rewrite cat_assoc.
+  rewrite compose_lift_ktree.
+  reflexivity.
+  typeclasses eauto.
+Qed.
+
+Fact lift_compose_ktree {A B C}: forall (f:A -> B) (bc: ktree E B C),
+    lift_ktree f >>> bc ⩯ fun a => bc (f a).
+Proof.
+  intros; intro a.
+  unfold lift_ktree, cat, Cat_ktree, ITree.cat.
+  rewrite bind_ret_. reflexivity.
+Qed.
+
+Fact compose_ktree_lift {A B C}: forall (ab: ktree E A B) (g:B -> C),
+    (ab >>> lift_ktree g)
+  ⩯ (fun a => ITree.map g (ab a)).
+Proof.
+  reflexivity.
+Qed.
+
+Lemma sym_ktree_unfold {A B}:
+  @lift_ktree E (A + B) (B + A) swap ⩯ swap.
+Proof.
+  intros []; reflexivity.
+Qed.
+
+End LiftLaws.
+
+Section MonoidalCategoryLaws.
+
+Context {E : Type -> Type}.
+
+Local Open Scope cat.
+
+Fact lift_case_sum {A B C} (ac : A -> C) (bc : B -> C) :
+    case_ (@lift_ktree E _ _ ac) (lift_ktree bc)
+  ⩯ lift_ktree (case_ ac bc).
+Proof.
+  intros []; reflexivity.
+Qed.
+
+(** *** [Unitors] lemmas *)
+
+(* This is probably generalizable into [Basics.Category]. *)
+
+Lemma unit_l_ktree (A : Type) :
+  unit_l ⩯ @lift_ktree E _ A unit_l.
+Proof.
+  intros [[]|]. reflexivity.
+Qed.
+
+Lemma unit_l'_ktree (A : Type) :
+  unit_l' ⩯ @lift_ktree E A (void + A) unit_l'.
+Proof.
+  reflexivity.
+Qed.
+
+Lemma unit_r_ktree (A : Type) :
+  unit_r ⩯ @lift_ktree E _ A unit_r.
+Proof.
+  intros [|[]]. reflexivity.
+Qed.
+
+Lemma unit_r'_ktree (A : Type) :
+  unit_r' ⩯ @lift_ktree E A (A + void) unit_r'.
+Proof.
+  reflexivity.
+Qed.
+
+Lemma case_l_ktree {A B: Type} (ab: @ktree E A (void + B)) :
+  ab >>> unit_l ⩯ (fun a: A => ITree.map unit_l (ab a)).
+Proof.
+  rewrite unit_l_ktree.
+  reflexivity.
+Qed.
+
+Lemma case_l_ktree' {A B: Type} (f: @ktree E (void + A) (void + B)) :
+  unit_l' >>> f ⩯ fun a => f (inr a).
+Proof.
+  rewrite unit_l'_ktree.
+  intro. unfold cat, Cat_ktree, ITree.cat, lift_ktree.
+  rewrite bind_ret_; reflexivity.
+Qed.
+
+Lemma case_r_ktree' {A B: Type} (f: @ktree E (A + void) (B + void)) :
+  unit_r' >>> f ⩯ fun a => f (inl a).
+Proof.
+  rewrite unit_r'_ktree.
+  intro. unfold cat, Cat_ktree, ITree.cat, lift_ktree.
+  rewrite bind_ret_; reflexivity.
+Qed.
+
+Lemma case_r_ktree {A B: Type} (ab: @ktree E A (B + void)) :
+  ab >>> unit_r ⩯ (fun a: A => ITree.map unit_r (ab a)).
+Proof.
+  rewrite unit_r_ktree.
+  reflexivity.
+Qed.
+
+(** *** [bimap] lemmas *)
+Local Opaque paco2.
+Local Opaque eutt loop ITree.bind'.
+
+Fact bimap_id_lift {A B C} (f : B -> C) :
+  bimap (id_ A) (@lift_ktree E _ _ f) ⩯ lift_ktree (bimap (id_ A) f).
+Proof.
+  unfold bimap, Bimap_Coproduct.
+  rewrite !cat_id_l, <- lift_case_sum, <- compose_lift_ktree.
+  reflexivity.
+  all: typeclasses eauto.
+Qed.
+
+Fact bimap_lift_id {A B C} (f : A -> B) :
+  bimap (@lift_ktree E _ _ f) (id_ C) ⩯ lift_ktree (bimap f id).
+Proof.
+  unfold bimap, Bimap_Coproduct.
+  rewrite !cat_id_l, <- lift_case_sum, <- compose_lift_ktree.
+  reflexivity.
+  all: typeclasses eauto.
+Qed.
+
+Global Instance Coproduct_ktree : Coproduct (ktree E) sum.
+Proof.
+  constructor.
+  - intros a b c f g.
+    unfold inl_, Inl_ktree.
+    rewrite lift_compose_ktree.
+    reflexivity.
+  - intros a b c f g.
+    unfold inr_, Inr_ktree.
+    rewrite lift_compose_ktree.
+    reflexivity.
+  - intros a b c f g fg Hf Hg [x | y].
+    + unfold inl_, Inl_ktree in Hf.
+      rewrite lift_compose_ktree in Hf.
+      specialize (Hf x). simpl in Hf. rewrite Hf. reflexivity.
+    + unfold inr_, Inr_ktree in Hg.
+      rewrite lift_compose_ktree in Hg.
+      specialize (Hg y). simpl in Hg. rewrite Hg. reflexivity.
+Qed.
+
+End MonoidalCategoryLaws.
